---
title: "Proof Methods"
date: 2026-02-14T18:59:00+03:00
author: "Selim Kaan Ã–zsoy, Middle East Technical University"
categories: ["Foundations of Mathematical Reasoning"]
draft: false
math: true
---


## Proof Methods and Strategies

### Formal Proof vs. Informal Proof
In mathematical practice, proofs are written in the daily English (informal), even though we have built a formal system to handle these. Why?
* Formal proofs are too long.
* Informal proofs are easier to read and communicate ideas.

However, every informal proof must be translatable into a formal proof.

Now, we shall learn various Proof Methods.

---

## 1. Direct Proof

Most mathematical statements are of the form $P \to Q$.

**Method:** Assume $P$ is true. Show that $Q$ is true using definitions, axioms, and previously proven theorems.

### Example: Parity of Product
**Proposition:** Let $m$ and $n$ be integers. If $m$ and $n$ are odd, then $mn$ is odd.

**Proof:**
Assume $m$ and $n$ are odd integers. By the definition of odd integers, there exists $k \in \mathbb{Z}$ such that $m = 2k+1$, and there exists $l \in \mathbb{Z}$ such that $n = 2l+1$. Since $k, l \in \mathbb{Z}$, setting $s = 2kl + k + l$. 

Hence,

$$
\begin{aligned}
mn &= (2k+1)(2l+1) \\\\
&= 4kl + 2k + 2l + 1 \\\\
&= 2(2kl + k + l) + 1 \\\\
&= 2s + 1
\end{aligned}
$$

For $s \in \mathbb{Z}$, $mn = 2s+1$. Hence, $mn$ is odd. 

---

## 2. Proof by Contrapositive

Given a statement of the form $P \to Q$. A proof by contrapositive of $P \to Q$ is a proof of the contrapositive statement $\neg Q \to \neg P$.

### Theorem
Let $n \in \mathbb{Z}$. If $n^2$ is odd, then $n$ is odd.

**Proof:**
We shall do a proof by contrapositive. Assume $n$ is not odd. Then $n$ is even. And so, there exists $k \in \mathbb{Z}$ such that $n = 2k$. Then:

$$
n^2 = (2k)^2 = 4k^2 = 2(2k^2).
$$

Since $k \in \mathbb{Z}$, let $m = 2k^2 \in \mathbb{Z}$. Hence, $n^2 = 2m$. Thus, $n^2$ is not odd (it is even). By contrapositive, if $n^2$ is odd, then $n$ is odd. $\square$

### Example 2
Let $p, q \in \mathbb{Z}^+$. If $n = pq$, then $p \le \sqrt{n}$ or $q \le \sqrt{n}$.

**Proof:**
We will prove by contrapositive. Suppose that $\neg (p \le \sqrt{n} \lor q \le \sqrt{n})$. This is equivalent to $p > \sqrt{n} \land q > \sqrt{n}$ (by De Morgan). Then:

$$
\begin{aligned}
& p \cdot q > \sqrt{n} \cdot \sqrt{n} = n \\\\
& p \cdot q > n
\end{aligned}
$$

Hence $n \neq pq$. Therefore, if $n = pq$, then $p \le \sqrt{n}$ or $q \le \sqrt{n}$. $\square$

---

## 3. Proof By Contradiction

In a proof by contradiction of a statement $P$, one assumes $\neg P$ (the negation of $P$) as hypothesis and works towards a contradiction (like $1=0$ or $Q \land \neg Q$). This shows that $P$ must be true. A typical format is as follows:

* **Theorem:** $P$.
* **Proof:** Assume towards a contradiction that $\neg P$.
* ... *(logical steps)* ...
* ... a contradiction.
* Then $P$. $\square$

### A Famous Example: Irrationality of $\sqrt{2}$
**Theorem:** $\sqrt{2}$ is irrational.

**Proof:**
Assume towards a contradiction that $\sqrt{2}$ is rational. Then $\sqrt{2} = \frac{m}{n}$ for some $m, n \in \mathbb{Z}$ with $\gcd(m,n) = 1$. (It follows that the fraction is in simplest form). Squaring both sides:

$$
2 = \frac{m^2}{n^2} \implies 2n^2 = m^2
$$

By Euclid's Lemma (or previous theorem), since $m^2$ is even ($2n^2$), $m$ must be even. So, $m = 2k$ for some $k \in \mathbb{Z}$. Substitute $m = 2k$ back into the equation:

$$
\begin{aligned}
2n^2 &= (2k)^2 \\\\
2n^2 &= 4k^2 \\\\
n^2 &= 2k^2
\end{aligned}
$$

Since $n^2 = 2k^2$, $n^2$ is even. By Euclid's Lemma, $n$ is even. So $n = 2l$ for some $l \in \mathbb{Z}$. But if $m$ is even and $n$ is even, then $2 \mid m$ and $2 \mid n$. So $\gcd(m,n) \ge 2$. This contradicts the assumption that $\gcd(m,n) = 1$. Hence $\sqrt{2}$ is irrational. $\square$

### Theorem: Infinitude of Primes
**Theorem:** There are infinitely many prime numbers.

**Proof:**
Suppose for a contradiction that there are finitely many prime numbers. Say, $p_1, p_2, \dots, p_k$ are all the prime numbers. Let $n = p_1 p_2 \dots p_k + 1$. By a theorem (Fundamental Theorem of Arithmetic), every integer must be divisible by a prime number. In particular, $n$ is divisible by a prime number $q$. Since $p_1, \dots, p_k$ are *all* primes, $q$ must be in the list $p_1, p_2, \dots, p_k$. So $q \mid n$ and $q \mid (n-1)$ (since $n-1 = p_1 \dots p_k$). Then $q \mid (n - (n-1)) \implies q \mid 1$. A contradiction. So there are infinitely many prime numbers. $\square$

---

## Case by Case Proofs

Given a statement $P$, a case-by-case proof of $P$ is done by splitting into cases covering all possibilities within a proof and obtaining the statement in each case separately.

$$
\begin{aligned}
& \text{Case I } - - - \text{ then } P. \\\\
& \text{Case II } - - - \text{ then } P. \\\\
& \vdots \\\\
& \text{Case X } - - - \text{ then } P.
\end{aligned}
$$

### Theorem (Monotonicity from Calculus)
**Theorem:** Let $f: \mathbb{R} \to \mathbb{R}$ be a differentiable function. Note that

$$
\text{sgn}(x) = \begin{cases} 
1 & \text{if } x > 0 \\\\
0 & \text{if } x = 0 \\\\
-1 & \text{if } x < 0 
\end{cases}
$$

If $\text{sgn}(f'(x))$ is the same for all $x \in \mathbb{R}$ (constant), then $f$ is monotone.

**Proof:**
Assume that $\text{sgn}(f'(x))$ is constant. We split into the following cases:

* **Case I:** $(\text{sgn}(f'(x)) = 1)$. In this case, $f'(x) > 0$ for all $x \in \mathbb{R}$. By a theorem from Calculus, $f$ must be increasing everywhere, if $a > b$, then $f(a) > f(b)$. Hence $f$ is monotone.
* **Case II:** $(\text{sgn}(f'(x)) = 0)$. In this case $f'(x) = 0$ for all $x \in \mathbb{R}$, then by a theorem, $f$ must be constant. However, constant functions are monotone.
* **Case III:** $(\text{sgn}(f'(x)) = -1)$. In this case $f'(x) < 0$ for all $x \in \mathbb{R}$. Then by a theorem, $f$ must be decreasing everywhere, therefore $f$ is monotone. This case cannot happen by the assumption if $f(x)$ is not constant. 

Hence, $f$ is monotone. $\square$

---

## Proofs of "If and only If" Statements

Given a statement of the form $P \iff Q$, one way to prove the statement(s) is to prove the statements $P \to Q$ and $Q \to P$ separately.

### Theorem (Absolute Values)
**Theorem:** Let $a, b$ be nonzero integers. Then,

$$
|a| = |b| \iff a = b \lor a = -b
$$

**Proof:**

**($\implies$) Direction:**
By contrapositive, suppose $a \neq b$ and $a \neq -b$. Then, $|a| \neq |b|$. We split into cases:
* **Case I:** $(|a| < |b|)$. In this case $|a| \neq |b|$.
* **Case II:** $(|a| > |b|)$. In this case $|a| \neq |b|$.

**($\impliedby$) Direction:**
Assume $a = b$ or $a = -b$. Then consider two cases:
* **Case I:** $(a = b)$. Then, since $a = b$, $|a| = |b|$.
* **Case II:** $(a = -b)$. Then, since $a = -b$, we have $|a| = |-b|$. Since $|-b| = |b|$ and $|a| = |-b| = |b|$. And so $|a| = |b|$.

Hence $|a| = |b|$. $\square$

---

## How to Prove Statements that involve Quantifiers

### Universal Statements
Given a statement of the form $\forall x \in A, P(x)$, one usually proves this statement by picking an **arbitrary** element $x \in A$ and then showing that $P(x)$ holds.

### Existential Statements
Given a statement of the form $\exists x \in A, P(x)$, we usually prove the statement by:
* **Construct/choose** an object $a \in A$, such that $P(a)$ holds.
* **Show** that such an object $a$ in $A$ with $P(a)$ holding exists.

**Theorem:** Let $a, b \in \mathbb{Z}^+$ be given. Then, there exists integers $q, r \in \mathbb{Z}$ such that $a = bq + r$ and $0 \leq r < b$.

### Theorem
For every positive integer $n$, there exists $a, b, c \in \mathbb{Z}^+$ such that $a^2 + b^2 = c^2$. 
*(Note: $\forall n \in \mathbb{N}, \exists a, b, c \in \mathbb{Z} \text{ s.t. } a^2+b^2=c^2 \land a,b,c > n$)*

**Proof:**
Let $n \in \mathbb{Z}^+$. Choose:
* $a = 2n + 1$
* $b = \frac{(2n+1)^2 - 1}{2}$
* $c = \frac{(2n+1)^2 + 1}{2}$

Since we have $a^2 + b^2 = c^2 \iff (c-b)(c+b) = a^2$, notice that $(c-b) = 1$ and $(c+b) = (2n+1)^2$. So $1 \cdot (2n+1)^2 = (2n+1)^2$. So $a^2 + b^2 = c^2$. 

Moreover, $a = 2n+1 > n$, and $b = \frac{(2n+1)^2 - 1}{2} = \frac{4n^2 + 4n}{2} = 2n^2 + 2n > n$. And $c = 2n^2 + 2n + 1 > n$. Then the theorem follows. $\square$

---

## How to Prove Equivalence of Several Statements

Given statements $P_1, P_2, \dots, P_n$, one way to prove that all these statements are logically equivalent is to prove the implications:

$$
P_1 \implies P_2, \quad P_2 \implies P_3, \quad \dots, \quad P_{n-1} \implies P_n, \quad P_n \implies P_1.
$$

### Example
Let $a, b \in \mathbb{Z}^+$. Then the following are equivalent (TFAE):
1. (i) $a$ and $b$ are relatively prime.
2. (ii) $a$ and $a+b$ are relatively prime.
3. (iii) $a$ and $a-b$ are relatively prime.

**Proof:**

* **$(i) \implies (ii)$:** By contrapositive, suppose $a$ and $a+b$ are not relatively prime. Then there exists $d = \gcd(a, a+b) \geq 2$. Then, by a theorem, $d \mid a$ and $d \mid a+b$, then $d \mid b$. Since $d \mid a$ and $d \mid b$ and $d \geq 2$, this means $a$ and $b$ are not relatively prime.
* **$(ii) \implies (iii)$:** By contrapositive, suppose $a$ and $a-b$ are not relatively prime. Then $\gcd(a, a-b) = d \geq 2$. For some $d \in \mathbb{Z}^+$. Since $d \mid a$ and $d \mid a-b$, then $d \mid a - (a-b) = b$. Since $d \mid a$ and $d \mid b$, then $d \mid a+b$. Then $\gcd(a, a+b) = d \geq 2$. So $a$ and $a+b$ are not relatively prime.
* **$(iii) \implies (i)$:** By contrapositive, suppose that $a$ and $b$ are not relatively prime. Then $d = \gcd(a, b) \geq 2$ for some $d \in \mathbb{Z}^+$. Then $d \mid a$ and $d \mid b$ and so $d \mid a-b$. Since $d \mid a-b$ and $d \mid a$ and $d \geq 2$, it follows that $\gcd(a-b, a) = d \geq 2$. So $a-b$ and $a$ are not relatively prime. $\square$

---

## Uniqueness Proofs

Given a statement of the form "There exists a unique $x \in A$ such that $P(x)$", one way to prove this statement is the following:

* **Step I:** **Prove** that such $x \in A$ exists. (**Existence**)
* **Step II:** **Put** two arbitrary $x, y \in A$ such that $P(x)$ and $P(y)$ and show that $x = y$.

$$
\exists! x \in A \quad P(x) \iff (\exists x \in A \quad P(x)) \land (\forall x, y \in A \quad (P(x) \land P(y) \to x = y))
$$

### Theorem
Let $a \ge 1$ be an integer. Then there exists a **unique** pair of positive integers $m, n$ such that 

$$
a = 2^m \cdot n \quad \text{and} \quad n \text{ is odd.}
$$

**Proof (Existence):**
Consider the set $S = \{ 2^k \mid k \in \mathbb{N} \text{ and } 2^k \mid a \}$. Since $2^0 = 1$ and $1 \mid a$, $S$ is non-empty. Since $S$ is a set of integers and it is bounded above (by $a$), then by the **Well Ordering Principle** (or its consequence), there exists a **largest** element.

Let $k_0$ be the **largest** element of $S$. Choose $m = k_0$. Then $2^m \mid a$. This means $a = 2^m \cdot n$ for some $n \in \mathbb{Z}^+$.

We claim that $n$ is odd. Suppose towards a contradiction that $n$ is even. If it were that $2 \mid n$, then we would have $n = 2l$ for some $l \in \mathbb{Z}^+$. Then:

$$
a = 2^m \cdot n = 2^m \cdot (2l) = 2^{m+1} \cdot l
$$

This implies $2^{m+1} \mid a$, which means $2^{m+1} \in S$. However, $2^{m+1} > 2^m$, which contradicts that $2^m$ is the **largest** element of $S$. Therefore, $n$ is not even, so $n$ is odd.  $\square$

{{< pdf "proof_methods.pdf">}}